%!TEX encoding = UTF-8 Unicode
\documentclass[11pt]{report}
\usepackage[margin = 1in]{geometry}

\usepackage{amsmath}
\usepackage{amssymb}
\usepackage{mleftright}
\usepackage{enumitem}
\usepackage{textcomp, gensymb}
\usepackage{tikz, tikz-cd}
\usepackage{bbding}
\usepackage{tabularx}
\usepackage{nicematrix}
\usepackage{extarrows}
\usepackage{lastpage}
\usepackage{hyperref}

\usepackage{fancyhdr}  % Header and Footer formatting

\usetikzlibrary{decorations.markings}

\usepackage{multicol}

\hypersetup{colorlinks = true,
            linkcolor = blue,
            citecolor = red,
            urlcolor = teal}

\pagestyle{fancy}
\renewcommand{\headrulewidth}{0.4pt}
\renewcommand{\footrulewidth}{0.4pt}
\setlength{\headheight}{18pt}

% Header and Footer Information
\lhead{\small\emph{Baitian Li}}
\chead{}
\rhead{\textsc{Complex Analysis}}
\lfoot{\today}
\cfoot{}
\rfoot{\thepage\ of \pageref{LastPage}}  % Counts the pages.

\makeatletter % This provides a total page count as \ref{NumPages}
\AtEndDocument{\immediate\write\@auxout{\string\newlabel{NumPages}{{\thepage}}}}
\makeatother

%\lineskiplimit=-\maxdimen\relax

\usepackage{amsthm}  % This will create the Problem environment
\newtheorem*{lemma}{Lemma}
\newtheorem*{theorem}{Theorem}
\newtheoremstyle{mythm}%
    {12pt}{}%
    {\sffamily}{}%
    {\bfseries \sffamily}{.}%
    {.5em}%
    {\thmname{#1}\thmnumber{ #2}\thmnote{ #3}}

\theoremstyle{mythm}

\expandafter\let\expandafter\oldproof\csname\string\proof\endcsname
\let\oldendproof\endproof
\renewenvironment{proof}[1][\proofname]{%
  \oldproof[\normalfont \bfseries #1]%
}{\oldendproof}

\renewcommand*{\proofname}{Proof}

\newtheoremstyle{myans}%
    {12pt}{}%
    {}{}%
    {\bfseries}{.}%
    {.5em}%
    {\thmname{#1}\thmnumber{ #2}\thmnote{ #3}}

\theoremstyle{myans}
\newtheorem*{answer}{Answer}

\setlist[enumerate]{noitemsep, topsep = 0.2em}
\setlist[enumerate]{label = {\bfseries \arabic*.}}
\setlist[enumerate, 2]{label = {(\alph*)}}
\setlist[description]{topsep = 0.2em, listparindent = \parindent, font = \normalfont,
  itemsep = 0em}

\newcommand{\mi}{\mathrm{i}}
\newcommand{\me}{\mathrm{e}}
\newcommand{\dd}{\mathop{}\!\mathrm{d}}

\newcommand{\bbC}{\mathbb{C}}
\newcommand{\bbD}{\mathbb{D}}
\newcommand{\bbR}{\mathbb{R}}

\newcommand{\norm}[1]{\|#1\|}

\renewcommand{\Re}{\operatorname{Re}}
\renewcommand{\Im}{\operatorname{Im}}

\DeclareMathOperator{\res}{res}

\allowdisplaybreaks

\begin{document}

\setcounter{chapter}{9}
\chapter{Applications of Theta Functions}

\section{Exercises}

\begin{enumerate}
  \item Prove that
  \[ \frac{(\Theta'(z|\tau))^2 - \Theta(z|\tau)\Theta''(z|\tau)}{\Theta(z|\tau)^2}
   = \wp_\tau(z - 1/2 - \tau / 2) + c_\tau, \]
  where $c_\tau$ can be expressed in terms of the first three derivatives of $\Theta(z|\tau)$, with respect
  to $z$, at $z = 1/2 + \tau/2$. Compare this formula with the result in Exercise 5 in the previous chapter.
  \begin{proof}
    We already know that LHS is $-(\log \Theta(z|\tau))''$, which has period $1$ and $\tau$.
    We know that the zeroes $\Theta(z|\tau)$ are exactly $(n+1/2) + (m+1/2)\tau$ with order 1,
    so the poles of $(\log \Theta(z|\tau))'$ are exactly at $(n+1/2) + (m+1/2)\tau$ with residue $1$.
    Thus we have
    \[ (\log \Theta(z|\tau))'' = - \frac 1{(z-1/2-\tau/2)^2} + c + \cdots \]
    near $z = 1/2 + \tau/2$, then $(\log \Theta(z|\tau))'' + \wp_\tau(z-1/2-\tau/2)$
    is holomorphic, thus is constant.

    Since $\wp_\tau(z) = z^{-2} + O(z^2)$, we have
    \[ -c_\tau = \lim_{z\to 1/2 + \tau/2} \left[ (\log \Theta(z|\tau))'' + \frac 1{(z+1/2+\tau/2)^2} \right]. \]
    Let $z_0 = 1/2 + \tau/2$, we have
    \[ f(z) = f'(z_0)(z-z_0) + \frac{f''(z_0)}2(z-z_0)^2 + \frac{f'''(z_0)}6(z-z_0)^2 + \cdots, \]
    thus
    \[ (\log f(z))' = \frac 1{z - z_0} + \frac{f''(z_0)}{2f'(z_0)} + \left(\frac{f'''(z_0)}{3f'(z_0)}
    - \frac{f''(z_0)^2}{4f'(z_0)^2}\right)(z-z_0) + \cdots, \]
    so
    \[ (\log f(z))'' = -\frac 1{(z-z_0)^2} + \left(\frac{f'''(z_0)}{3f'(z_0)}
    - \frac{f''(z_0)^2}{4f'(z_0)^2}\right)+\cdots, \]
    then we have
    \[ (\log \Theta(z|\tau))'' + \wp_\tau(z - z_0) = \frac{\Theta'''(z_0|\tau)}{3\Theta'(z_0|\tau)}
    - \frac{\Theta''(z_0|\tau)^2}{4\Theta'(z_0|\tau)^2}. \qedhere  \]
  \end{proof}
  \setcounter{enumi}{4}
  \item Let
  \[ F(x) = \sum_{n=0}^\infty p(n)x^n = \prod_{n=1}^\infty \frac 1{1-x^n} \]
  be the generating function for the partitions. Show that
  \begin{center}
    $\displaystyle \log F(x) \sim \frac{\pi^2}{6(1-x)}$ \quad
    as $x\to 1$, with $0<x<1$.
  \end{center}
  \begin{proof}
    When $|x|<1$, we have the absolute convergence
    \begin{align*}
      \log F(x) &= \sum_{n=1}^\infty \log \frac 1{1-x^n}\\
      &= \sum_{n=1}^\infty \sum_{m=1}^\infty \frac{x^{nm}}{m}\\
      &= \sum_{m=1}^\infty \frac 1{m} \frac{x^m}{1-x^m},
    \end{align*}
    then we have
    \begin{align*}
      (1-x)\log F(x) &= \sum_{m=1}^\infty \frac 1{m} \frac{x^m (1-x)}{1-x^m},
    \end{align*}
    note that on $(0, 1)$,
    \begin{align*}
      \left(\frac{x^m(1-x)}{1-x^m}\right)' &= \frac{x^{m-1}(m-(m+1)x+x^m)}{(1-x^m)^2}\\
      &= \frac{x^{m-1}(1-x)}{(1-x^m)^2}\left(m - \frac{x-x^m}{1-x}\right)\\
      &= \frac{x^{m-1}(1-x)}{(1-x^m)^2}\left((1 - x) + (1-x^2) + \cdots + (1-x^m)\right) \geq 0,
    \end{align*}
    so the function is increasing. We have
    \begin{align*}
      \lim_{x\to 1} (1-x)\log F(x) &= \sum_{m=1}^\infty \frac 1 m \lim_{x\to 1} \frac{x^m(1-x)}{1-x^m}\\
      &= \sum_{m=1}^\infty \frac 1{m^2}\\
      &= \zeta(2) = \frac{\pi^2} 6 .
    \end{align*}
    Thus $\log F(x) \sim \pi^2 / 6(1-x)$ at $x\to 1$.
  \end{proof}
\end{enumerate}

\end{document}
